% ====   Order pq   ====
\section{Groups of Order \(pq\)}
Let \(G\) be a group of order \(pq\) where \(p\), \(q\) are prime numbers with \(p > q\), and let \(n_p\) and \(n_q\)
denote the number of Sylow p-subgroups and Sylow q-subgroups of \(G\) respectively.
Then by Sylow's~Theorems:
\[n_p \equiv 1 \ \pmod{p} \quad \text{and} \quad n_p \mid q\]
So \(G\) has a unique Sylow \(p\)-subgroup, say \(P \nrmsgp G\), and a Sylow \(q\)-subgroup, \(Q \leqslant G\).
Because \(p\) and \(q\) are prime numbers, \(P \cong C_p\) and \(Q \cong C_q\).
Pick generators for each, say \(\langle x \rangle  = P\) and \(\langle y \rangle = Q\).
We have 2 possibilities for \(n_q\): \(p-1\) is a multiple of \(q\) or 1.

\begin{enumerate}[\bfseries{Case} 1:]
    \item \(q \nmid p - 1\).

        If \(p-1\) \emph{is not} a multiple of \(q\) then \(n_q = 1\) and \(Q \nrmsgp G\), hence:
        \[G = P \times Q \cong C_{pq}\]
    \item \( q \mid p - 1\).

        If \(p-1\) \emph{is} a multiple of \(q\) then \(n_q = p\) and so \(Q\) is \emph{not} normal in \(G\).
        By Lagrange's Theorem, \(P \cap Q = \bm{1}\) and by Lemma~\ref{lem:setprodorder}, \(|PQ| = pq\).
        Hence, as well as the direct product, we have \(G = P \rtimes Q\), some non-trivial semidirect product.

        By Lemma~\ref{lem:aut}, \(\Aut{C_p} \cong \units{p} \cong C_{p-1}\).
        So if \(\nu \in \units{p}\), then \(x \mapsto x^\nu\) is an automorphism.
        We know also that \(C_{p-1}\) has a unique subgroup of order \(q\),
        hence \(G\) has the presentation:
        \[G = \langle \, x, y, \mid x^p = y^q = 1,\ y^{-1}xy = x^a \, \rangle\]
        where \(a\) is a generator for the subgroup of order \(q\) in \(\units{p}\).

        Notice that picking different generators are equivalent up to isomorphism because the composition of two
        isomorphisms is an isomorphism.
\end{enumerate}

\begin{mdframed}[align=center,nobreak=true]
    \begin{center}
        Any group of order \(pq\) is isomorphic to one of:
        \[C_{pq}\]
        \[\gen{x, y \mid x^p = y^q = 1,\ y^{-1}xy = x^a} \tag{additionally, if \(q \mid p-1\)}\]
    \end{center}
\end{mdframed}
